feat: theorify Value

GroupoidModel/Syntax/Typechecker/Value.lean
@@ -2,6 +2,8 @@ import GroupoidModel.Syntax.GCongr
 import GroupoidModel.Syntax.Injectivity
 import GroupoidModel.Syntax.Synth
 
+variable {χ : Type*} {E : Env χ}
+
 /-! # Values, neutral forms, closures, and evaluation environments
 
 This module sets up definitions for normalization by evaluation (NbE).
@@ -15,6 +17,8 @@ attribute [local grind]
   EqTm.refl_tm EqTm.symm_tm EqTm.trans_tm
 
 mutual
+variable (χ : Type*)
+
 /-- Values are produced by the evaluator during NbE.
 
 The value type is obtained by:
@@ -84,14 +88,16 @@ In some NbE implementations, this would be a meta-level closure `Expr → Expr`;
 the present variant is a defunctionalization due to Abel. -/
 inductive Clos where
   | of_val (env : List Val) (v : Val)
-  | of_expr (env : List Val) (t : Expr)
+  | of_expr (env : List Val) (t : Expr χ)
   deriving Inhabited
 end
 
 /-! ## Relation of values to terms -/
 
 mutual
-inductive ValEqTp : Ctx → Nat → Val → Expr → Prop
+variable (E : Env χ)
+
+inductive ValEqTp : Ctx χ → Nat → Val χ → Expr χ → Prop
   | pi {Γ vA A vB B l l'} :
     ValEqTp Γ l vA A →
     ClosEqTp Γ l l' A vB B →
@@ -106,7 +112,7 @@ inductive ValEqTp : Ctx → Nat → Val → Expr → Prop
     ValEqTm Γ l vu u A →
     ValEqTp Γ l (.Id l vA vt vu) (.Id l A t u)
   | univ {Γ l} :
-    WfCtx Γ →
+    WfCtx E Γ →
     l < univMax →
     ValEqTp Γ (l + 1) (.univ l) (.univ l)
   | el {Γ na a l} :
@@ -114,18 +120,18 @@ inductive ValEqTp : Ctx → Nat → Val → Expr → Prop
     ValEqTp Γ l (.el na) (.el a)
   | conv_tp {Γ vA A A' l} :
     ValEqTp Γ l vA A →
-    Γ ⊢[l] A ≡ A' →
+    E ∣ Γ ⊢[l] A ≡ A' →
     ValEqTp Γ l vA A'
 
 -- Note: neutral types are embedded in `Val` directly and don't need a `NeutEqTp` relation.
 
-inductive ValEqTm : Ctx → Nat → Val → Expr → Expr → Prop
+inductive ValEqTm : Ctx χ → Nat → Val χ → Expr χ → Expr χ → Prop
   | lam {Γ A B vA vb b l l'} :
     ValEqTp Γ l vA A →
     ClosEqTm Γ l l' A B vb b →
     ValEqTm Γ (max l l') (.lam l l' vA vb) (.lam l l' A b) (.pi l l' A B)
   | pair {Γ A B vt t vu u l l'} :
-    (A, l) :: Γ ⊢[l'] B →
+    E ∣ (A, l) :: Γ ⊢[l'] B →
     ValEqTm Γ l vt t A →
     ValEqTm Γ l' vu u (B.subst t.toSb) →
     ValEqTm Γ (max l l') (.pair l l' vt vu) (.pair l l' B t u) (.sigma l l' A B)
@@ -142,13 +148,13 @@ inductive ValEqTm : Ctx → Nat → Val → Expr → Expr → Prop
     ValEqTm Γ l (.neut vn vA) n A
   | conv_nf {Γ A A' vt t t' l} :
     ValEqTm Γ l vt t A →
-    Γ ⊢[l] t ≡ t' : A →
-    Γ ⊢[l] A ≡ A' →
+    E ∣ Γ ⊢[l] t ≡ t' : A →
+    E ∣ Γ ⊢[l] A ≡ A' →
     ValEqTm Γ l vt t' A'
 
-inductive NeutEqTm : Ctx → Nat → Neut → Expr → Expr → Prop
+inductive NeutEqTm : Ctx χ → Nat → Neut χ → Expr χ → Expr χ → Prop
   | bvar {Γ A i l} :
-    WfCtx Γ →
+    WfCtx E Γ →
     Lookup Γ i A l →
     NeutEqTm Γ l (.bvar (Γ.length - i - 1)) (.bvar i) A
   | app {Γ vA A B vf f va a l l'} :
@@ -171,89 +177,89 @@ inductive NeutEqTm : Ctx → Nat → Neut → Expr → Expr → Prop
     NeutEqTm Γ l' (.idRec l l' vA va cM vr nh) (.idRec l l' a M r b h) (M.subst (.snoc b.toSb h))
   | conv_neut {Γ A A' vn n n' l} :
     NeutEqTm Γ l vn n A →
-    Γ ⊢[l] n ≡ n' : A →
-    Γ ⊢[l] A ≡ A' →
+    E ∣ Γ ⊢[l] n ≡ n' : A →
+    E ∣ Γ ⊢[l] A ≡ A' →
     NeutEqTm Γ l vn n' A'
 
 /-- `ClosEqTp Δ l l' A vB B` -/
-inductive ClosEqTp : Ctx → Nat → Nat → Expr → Clos → Expr → Prop
+inductive ClosEqTp : Ctx χ → Nat → Nat → Expr χ → Clos χ → Expr χ → Prop
   | clos_tp {Δ Γ A B Aenv env σ l l'} :
     EnvEqSb Δ env σ Γ →
     -- The equality argument builds in conversion.
-    Δ ⊢[l] A.subst σ ≡ Aenv →
-    (A, l) :: Γ ⊢[l'] B →
+    E ∣ Δ ⊢[l] A.subst σ ≡ Aenv →
+    E ∣ (A, l) :: Γ ⊢[l'] B →
     ClosEqTp Δ l l' Aenv (.of_expr env B) (B.subst <| Expr.up σ)
   | clos_val_tp {Δ Γ A B Aenv vB env σ l l'} :
     EnvEqSb Δ env σ Γ →
-    Δ ⊢[l] A.subst σ ≡ Aenv →
+    E ∣ Δ ⊢[l] A.subst σ ≡ Aenv →
     ValEqTp ((A, l) :: Γ) l' vB B →
     ClosEqTp Δ l l' Aenv (.of_val env vB) (B.subst <| Expr.up σ)
 
 /- Can `ClosEqTp` and `Clos₂EqTp` be subsumed by `ClosₙEqTp` that takes a context?
 Would need defining substitution on contexts, and `Expr.upN`. -/
-inductive Clos₂EqTp : Ctx → Expr → Nat → Expr → Nat → Nat → Clos → Expr → Prop
+inductive Clos₂EqTp : Ctx χ → Expr χ → Nat → Expr χ → Nat → Nat → Clos χ → Expr χ → Prop
   | clos₂_tp {Δ Γ A B C Aenv Benv env σ l l' l''} :
     EnvEqSb Δ env σ Γ →
-    Δ ⊢[l] A.subst σ ≡ Aenv →
-    (Aenv, l) :: Δ ⊢[l'] B.subst (Expr.up σ) ≡ Benv →
-    (B, l') :: (A, l) :: Γ ⊢[l''] C →
+    E ∣ Δ ⊢[l] A.subst σ ≡ Aenv →
+    E ∣ (Aenv, l) :: Δ ⊢[l'] B.subst (Expr.up σ) ≡ Benv →
+    E ∣ (B, l') :: (A, l) :: Γ ⊢[l''] C →
     Clos₂EqTp Δ Aenv l Benv l' l'' (.of_expr env C) (C.subst <| Expr.up <| Expr.up σ)
   | clos₂_val_tp {Δ Γ A B C vC Aenv Benv env σ l l' l''} :
     EnvEqSb Δ env σ Γ →
-    Δ ⊢[l] A.subst σ ≡ Aenv →
-    (Aenv, l) :: Δ ⊢[l'] B.subst (Expr.up σ) ≡ Benv →
+    E ∣ Δ ⊢[l] A.subst σ ≡ Aenv →
+    E ∣ (Aenv, l) :: Δ ⊢[l'] B.subst (Expr.up σ) ≡ Benv →
     ValEqTp ((B, l') :: (A, l) :: Γ) l'' vC C →
     Clos₂EqTp Δ Aenv l Benv l' l'' (.of_val env vC) (C.subst <| Expr.up <| Expr.up σ)
 
 /-- `ClosEqTm Δ l l' A B vb b` -/
-inductive ClosEqTm : Ctx → Nat → Nat → Expr → Expr → Clos → Expr → Prop
+inductive ClosEqTm : Ctx χ → Nat → Nat → Expr χ → Expr χ → Clos χ → Expr χ → Prop
   | clos_tm {Δ Γ A B Aenv Benv b env σ l l'} :
     EnvEqSb Δ env σ Γ →
-    Δ ⊢[l] A.subst σ ≡ Aenv →
-    (Aenv, l) :: Δ ⊢[l'] (B.subst <| Expr.up σ) ≡ Benv →
-    (A, l) :: Γ ⊢[l'] b : B →
+    E ∣ Δ ⊢[l] A.subst σ ≡ Aenv →
+    E ∣ (Aenv, l) :: Δ ⊢[l'] (B.subst <| Expr.up σ) ≡ Benv →
+    E ∣ (A, l) :: Γ ⊢[l'] b : B →
     ClosEqTm Δ l l' Aenv Benv (.of_expr env b) (b.subst <| Expr.up σ)
   | clos_val_tm {Δ Γ A B Aenv Benv b vb env σ l l'} :
     EnvEqSb Δ env σ Γ →
-    Δ ⊢[l] A.subst σ ≡ Aenv →
-    (Aenv, l) :: Δ ⊢[l'] (B.subst <| Expr.up σ) ≡ Benv →
+    E ∣ Δ ⊢[l] A.subst σ ≡ Aenv →
+    E ∣ (Aenv, l) :: Δ ⊢[l'] (B.subst <| Expr.up σ) ≡ Benv →
     ValEqTm ((A, l) :: Γ) l' vb b B →
     ClosEqTm Δ l l' Aenv Benv (.of_val env vb) (b.subst <| Expr.up σ)
 
-inductive EnvEqSb : Ctx → List Val → (Nat → Expr) → Ctx → Prop
+inductive EnvEqSb : Ctx χ → List (Val χ) → (Nat → Expr χ) → Ctx χ → Prop
   /- Possible optimization: allow `EnvEqSb Γ [] Expr.bvar Γ`
   and replace `envOfLen ‖Γ‖` by `[]`. -/
-  | nil {Γ} (σ) : WfCtx Γ → EnvEqSb Γ [] σ []
-  | snoc {Δ Γ A vt t E σ l} :
-    EnvEqSb Δ E σ Γ →
-    Γ ⊢[l] A →
+  | nil {Γ} (σ) : WfCtx E Γ → EnvEqSb Γ [] σ []
+  | snoc {Δ Γ A vt t Eᵥ σ l} :
+    EnvEqSb Δ Eᵥ σ Γ →
+    E ∣ Γ ⊢[l] A →
     ValEqTm Δ l vt t (A.subst σ) →
-    EnvEqSb Δ (vt :: E) (Expr.snoc σ t) ((A, l) :: Γ)
+    EnvEqSb Δ (vt :: Eᵥ) (Expr.snoc σ t) ((A, l) :: Γ)
 end
 
 /-! ## Well-formed evaluation environments -/
 
 namespace EnvEqSb
 
-theorem wf_dom : ∀ {Δ E σ Γ}, EnvEqSb Δ E σ Γ → WfCtx Δ := by
+theorem wf_dom : ∀ {Δ Eᵥ σ Γ}, EnvEqSb E Δ Eᵥ σ Γ → WfCtx E Δ := by
   mutual_induction EnvEqSb
   all_goals grind
 
-theorem wf_cod : ∀ {Δ E σ Γ}, EnvEqSb Δ E σ Γ → WfCtx Γ := by
+theorem wf_cod : ∀ {Δ Eᵥ σ Γ}, EnvEqSb E Δ Eᵥ σ Γ → WfCtx E Γ := by
   mutual_induction EnvEqSb
   all_goals grind [WfCtx.nil, WfCtx.snoc]
 
-theorem eq_length : ∀ {Δ E σ Γ}, EnvEqSb Δ E σ Γ → E.length = Γ.length := by
+theorem eq_length : ∀ {Δ Eᵥ σ Γ}, EnvEqSb E Δ Eᵥ σ Γ → Eᵥ.length = Γ.length := by
   mutual_induction EnvEqSb
   all_goals intros; try exact True.intro
   all_goals simp; try grind
 
-theorem lookup_lt {Δ Γ E σ i A l} : EnvEqSb Δ E σ Γ → Lookup Γ i A l → i < E.length :=
+theorem lookup_lt {Δ Γ Eᵥ σ i A l} : EnvEqSb E Δ Eᵥ σ Γ → Lookup Γ i A l → i < Eᵥ.length :=
   fun env lk => env.eq_length ▸ lk.lt_length
 
-theorem lookup_eq : ∀ {Δ E σ Γ}, (env : EnvEqSb Δ E σ Γ) →
+theorem lookup_eq : ∀ {Δ Eᵥ σ Γ}, (env : EnvEqSb E Δ Eᵥ σ Γ) →
     ∀ {A i l}, (lk : Lookup Γ i A l) →
-    ValEqTm Δ l (E[i]'(env.lookup_lt lk)) (σ i) (A.subst σ) := by
+    ValEqTm E Δ l (Eᵥ[i]'(env.lookup_lt lk)) (σ i) (A.subst σ) := by
   mutual_induction EnvEqSb
   all_goals intros; try exact True.intro
   case nil lk => cases lk
@@ -262,13 +268,15 @@ theorem lookup_eq : ∀ {Δ E σ Γ}, (env : EnvEqSb Δ E σ Γ) →
     . exact autosubst% v
     . exact autosubst% ih lk
 
-lemma Expr.eq_snoc_get_zero (σ : Nat → Expr) : σ = Expr.snoc (Expr.comp σ Expr.wk) (σ 0) := by
+private lemma Expr.eq_snoc_get_zero (σ : Nat → Expr χ) :
+    σ = Expr.snoc (Expr.comp σ Expr.wk) (σ 0) := by
   ext i; cases i <;> rfl
 
-theorem mk : ∀ {Γ}, WfCtx Γ → ∀ {Δ} {E : List Val} {σ}, WfCtx Δ → (eq : Γ.length = E.length) →
+theorem mk : ∀ {Γ}, WfCtx E Γ → ∀ {Δ} {Eᵥ : List (Val χ)} {σ},
+    WfCtx E Δ → (eq : Γ.length = Eᵥ.length) →
     (∀ {i A l}, (lk : Lookup Γ i A l) →
-      ValEqTm Δ l (E[i]'(eq ▸ lk.lt_length)) (σ i) (A.subst σ)) →
-    EnvEqSb Δ E σ Γ := by
+      ValEqTm E Δ l (Eᵥ[i]'(eq ▸ lk.lt_length)) (σ i) (A.subst σ)) →
+    EnvEqSb E Δ Eᵥ σ Γ := by
   mutual_induction WfCtx
   all_goals intros; try exact True.intro
   case nil eq _ =>
@@ -289,33 +297,20 @@ end EnvEqSb
 
 /-! ## Values are well-typed as expressions -/
 
+variable [Fact E.Wf]
+
 theorem wf_expr :
-    (∀ {Γ l vA A}, ValEqTp Γ l vA A → Γ ⊢[l] A) ∧
-    (∀ {Γ l vt t A}, ValEqTm Γ l vt t A → Γ ⊢[l] t : A) ∧
-    (∀ {Γ l vt t A}, NeutEqTm Γ l vt t A → Γ ⊢[l] t : A) ∧
-    (∀ {Γ l l' A vB B}, ClosEqTp Γ l l' A vB B → (A, l) :: Γ ⊢[l'] B) ∧
-    (∀ {Γ A l B l' l'' cC C}, Clos₂EqTp Γ A l B l' l'' cC C → (B, l') :: (A, l) :: Γ ⊢[l''] C) ∧
-    (∀ {Γ l l' A B vb b}, ClosEqTm Γ l l' A B vb b → (A, l) :: Γ ⊢[l'] b : B) ∧
-    (∀ {Γ E σ Γ'}, EnvEqSb Γ E σ Γ' → WfSb Γ σ Γ') := by
+    (∀ {Γ l vA A}, ValEqTp E Γ l vA A → E ∣ Γ ⊢[l] A) ∧
+    (∀ {Γ l vt t A}, ValEqTm E Γ l vt t A → E ∣ Γ ⊢[l] t : A) ∧
+    (∀ {Γ l vt t A}, NeutEqTm E Γ l vt t A → E ∣ Γ ⊢[l] t : A) ∧
+    (∀ {Γ l l' A vB B}, ClosEqTp E Γ l l' A vB B → E ∣ (A, l) :: Γ ⊢[l'] B) ∧
+    (∀ {Γ A l B l' l'' cC C}, Clos₂EqTp E Γ A l B l' l'' cC C → E ∣ (B, l') :: (A, l) :: Γ ⊢[l''] C) ∧
+    (∀ {Γ l l' A B vb b}, ClosEqTm E Γ l l' A B vb b → E ∣ (A, l) :: Γ ⊢[l'] b : B) ∧
+    (∀ {Γ Eᵥ σ Γ'}, EnvEqSb E Γ Eᵥ σ Γ' → WfSb E Γ σ Γ') := by
   mutual_induction ValEqTp
   all_goals dsimp; intros
-  case pi => grind [WfTp.pi]
-  case sigma => grind [WfTp.sigma]
-  case univ => grind [WfTp.univ]
-  case Id => grind [WfTp.Id]
-  case el => grind [WfTp.el]
   case conv_tp => grind [EqTp.wf_right]
-  case lam => grind [WfTm.lam]
-  case pair => grind [WfTm.pair]
-  case refl => grind [WfTm.refl]
-  case code => grind [WfTm.code]
-  case neut_tm => grind
   case conv_nf tt' AA' _ => exact tt'.wf_right.conv AA'
-  case bvar Γ lk => exact WfTm.bvar Γ lk
-  case app => grind [WfTm.app]
-  case fst => grind [WfTm.fst]
-  case snd => grind [WfTm.snd]
-  case idRec => grind [WfTm.idRec]
   case conv_neut nn' AA' _ => exact nn'.wf_right.conv AA'
   case clos₂_tp Aenv Benv C σ =>
     have B := C.wf_binder
@@ -346,90 +341,76 @@ theorem wf_expr :
     have := this.conv_ctx (EqCtx.refl Aenv.wf_ctx |>.snoc Aenv)
     exact this.conv Benv
   case nil => apply WfSb.terminal; assumption
-  case snoc => grind [WfSb.snoc]
+  grind_cases
 
-theorem ValEqTp.wf_tp {Γ l vA A} (h : ValEqTp Γ l vA A) : Γ ⊢[l] A :=
+theorem ValEqTp.wf_tp {Γ l vA A} (h : ValEqTp E Γ l vA A) : E ∣ Γ ⊢[l] A :=
   _root_.wf_expr.1 h
 
-theorem ValEqTm.wf_tm {Γ l vt t A} (h : ValEqTm Γ l vt t A) : Γ ⊢[l] t : A :=
+theorem ValEqTm.wf_tm {Γ l vt t A} (h : ValEqTm E Γ l vt t A) : E ∣ Γ ⊢[l] t : A :=
   _root_.wf_expr.2.1 h
 
-theorem NeutEqTm.wf_tm {Γ l vt t A} (h : NeutEqTm Γ l vt t A) : Γ ⊢[l] t : A :=
+theorem NeutEqTm.wf_tm {Γ l vt t A} (h : NeutEqTm E Γ l vt t A) : E ∣ Γ ⊢[l] t : A :=
   _root_.wf_expr.2.2.1 h
 
-theorem ClosEqTp.wf_tp {Γ l l' A vB B} (h : ClosEqTp Γ l l' A vB B) :
-    (A, l) :: Γ ⊢[l'] B :=
+theorem ClosEqTp.wf_tp {Γ l l' A vB B} (h : ClosEqTp E Γ l l' A vB B) :
+    E ∣ (A, l) :: Γ ⊢[l'] B :=
   _root_.wf_expr.2.2.2.1 h
 
-theorem Clos₂EqTp.wf_tp {Γ A B C vC l l' l''} (h : Clos₂EqTp Γ A l B l' l'' vC C) :
-    (B, l') :: (A, l) :: Γ ⊢[l''] C :=
+theorem Clos₂EqTp.wf_tp {Γ A B C vC l l' l''} (h : Clos₂EqTp E Γ A l B l' l'' vC C) :
+    E ∣ (B, l') :: (A, l) :: Γ ⊢[l''] C :=
   _root_.wf_expr.2.2.2.2.1 h
 
-theorem ClosEqTm.wf_tm {Γ l l' A B vb b} (h : ClosEqTm Γ l l' A B vb b) :
-    (A, l) :: Γ ⊢[l'] b : B :=
+theorem ClosEqTm.wf_tm {Γ l l' A B vb b} (h : ClosEqTm E Γ l l' A B vb b) :
+    E ∣ (A, l) :: Γ ⊢[l'] b : B :=
   _root_.wf_expr.2.2.2.2.2.1 h
 
-theorem EnvEqSb.wf_sb {Δ E σ Γ} (h : EnvEqSb Δ E σ Γ) : WfSb Δ σ Γ :=
+theorem EnvEqSb.wf_sb {Δ Eᵥ σ Γ} (h : EnvEqSb E Δ Eᵥ σ Γ) : WfSb E Δ σ Γ :=
   _root_.wf_expr.2.2.2.2.2.2 h
 
 theorem ValEqTm.conv_tm {Γ A vt t t' l} :
-    ValEqTm Γ l vt t A → Γ ⊢[l] t ≡ t' : A → ValEqTm Γ l vt t' A :=
+    ValEqTm E Γ l vt t A → E ∣ Γ ⊢[l] t ≡ t' : A → ValEqTm E Γ l vt t' A :=
   fun h eq => h.conv_nf eq (EqTp.refl_tp eq.wf_tp)
 
 theorem ValEqTm.conv_tp {Γ A A' vt t l} :
-    ValEqTm Γ l vt t A → Γ ⊢[l] A ≡ A' → ValEqTm Γ l vt t A' :=
+    ValEqTm E Γ l vt t A → E ∣ Γ ⊢[l] A ≡ A' → ValEqTm E Γ l vt t A' :=
   fun h eq => h.conv_nf (EqTm.refl_tm h.wf_tm) eq
 
 theorem NeutEqTm.conv_tm {Γ A vt t t' l} :
-    NeutEqTm Γ l vt t A → Γ ⊢[l] t ≡ t' : A → NeutEqTm Γ l vt t' A :=
+    NeutEqTm E Γ l vt t A → E ∣ Γ ⊢[l] t ≡ t' : A → NeutEqTm E Γ l vt t' A :=
   fun h eq => h.conv_neut eq (EqTp.refl_tp eq.wf_tp)
 
 theorem NeutEqTm.conv_tp {Γ A A' vt t l} :
-    NeutEqTm Γ l vt t A → Γ ⊢[l] A ≡ A' → NeutEqTm Γ l vt t A' :=
+    NeutEqTm E Γ l vt t A → E ∣ Γ ⊢[l] A ≡ A' → NeutEqTm E Γ l vt t A' :=
   fun h eq => h.conv_neut (EqTm.refl_tm h.wf_tm) eq
 
 /-! ## Values are closed under context conversion -/
 
-attribute [local grind ←] EqCtx.length_eq in
-attribute [local grind →] WfTp.conv_ctx EqTp.conv_ctx WfTm.conv_ctx EqTm.conv_ctx in
+attribute [local grind →] EqCtx.length_eq WfTp.conv_ctx EqTp.conv_ctx WfTm.conv_ctx EqTm.conv_ctx in
 theorem conv_ctx :
-    (∀ {Γ l vA A}, ValEqTp Γ l vA A → ∀ {Γ'}, EqCtx Γ Γ' → ValEqTp Γ' l vA A) ∧
-    (∀ {Γ l vt t A}, ValEqTm Γ l vt t A → ∀ {Γ'}, EqCtx Γ Γ' → ValEqTm Γ' l vt t A) ∧
-    (∀ {Γ l vt t A}, NeutEqTm Γ l vt t A → ∀ {Γ'}, EqCtx Γ Γ' → NeutEqTm Γ' l vt t A) ∧
-    (∀ {Γ l l' A vB B}, ClosEqTp Γ l l' A vB B → ∀ {Γ'}, EqCtx Γ Γ' → ClosEqTp Γ' l l' A vB B) ∧
-    (∀ {Γ A l B l' l'' vC C}, Clos₂EqTp Γ A l B l' l'' vC C →
-      ∀ {Γ'}, EqCtx Γ Γ' → Clos₂EqTp Γ' A l B l' l'' vC C) ∧
-    (∀ {Γ l l' A B vb b}, ClosEqTm Γ l l' A B vb b → ∀ {Γ'}, EqCtx Γ Γ' →
-      ClosEqTm Γ' l l' A B vb b) ∧
-    (∀ {Γ E σ Δ}, EnvEqSb Γ E σ Δ → ∀ {Γ'}, EqCtx Γ Γ' → EnvEqSb Γ' E σ Δ) := by
+    (∀ {Γ l vA A}, ValEqTp E Γ l vA A → ∀ {Γ'},
+      EqCtx E Γ Γ' → ValEqTp E Γ' l vA A) ∧
+    (∀ {Γ l vt t A}, ValEqTm E Γ l vt t A → ∀ {Γ'},
+      EqCtx E Γ Γ' → ValEqTm E Γ' l vt t A) ∧
+    (∀ {Γ l vt t A}, NeutEqTm E Γ l vt t A → ∀ {Γ'},
+      EqCtx E Γ Γ' → NeutEqTm E Γ' l vt t A) ∧
+    (∀ {Γ l l' A vB B}, ClosEqTp E Γ l l' A vB B → ∀ {Γ'},
+      EqCtx E Γ Γ' → ClosEqTp E Γ' l l' A vB B) ∧
+    (∀ {Γ A l B l' l'' vC C}, Clos₂EqTp E Γ A l B l' l'' vC C →
+      ∀ {Γ'}, EqCtx E Γ Γ' → Clos₂EqTp E Γ' A l B l' l'' vC C) ∧
+    (∀ {Γ l l' A B vb b}, ClosEqTm E Γ l l' A B vb b → ∀ {Γ'}, EqCtx E Γ Γ' →
+      ClosEqTm E Γ' l l' A B vb b) ∧
+    (∀ {Γ Eᵥ σ Δ}, EnvEqSb E Γ Eᵥ σ Δ → ∀ {Γ'}, EqCtx E Γ Γ' → EnvEqSb E Γ' Eᵥ σ Δ) := by
   mutual_induction ValEqTp
   all_goals intros
-  case pi => grind [ValEqTp.pi]
-  case sigma => grind [ValEqTp.sigma]
-  case Id => grind [ValEqTp.Id]
   case univ => grind [ValEqTp.univ, EqCtx.wf_right]
-  case el => grind [ValEqTp.el]
-  case conv_tp => grind [ValEqTp.conv_tp]
-  case lam eq => grind [ValEqTm.lam]
   case pair B _ _ _ _ _ eq =>
     apply ValEqTm.pair (B.conv_ctx (eq.snoc <| EqTp.refl_tp B.wf_binder)) <;> grind
-  case refl => grind [ValEqTm.refl]
-  case code => grind [ValEqTm.code]
-  case neut_tm => grind [ValEqTm.neut_tm]
-  case conv_nf => grind [ValEqTm.conv_nf]
   case bvar lk _ eq =>
     have ⟨A', _, lk'⟩ := Lookup.of_lt_length <| eq.length_eq ▸ lk.lt_length
     obtain ⟨rfl, eqA⟩ := eq.lookup_eq lk lk'
     have := NeutEqTm.bvar eq.wf_right lk'
     rw [eq.length_eq]
     exact NeutEqTm.conv_neut this (EqTm.refl_tm this.wf_tm) (eqA.symm_tp.conv_ctx eq)
-  case app eq => grind [NeutEqTm.app]
-  case fst => grind [NeutEqTm.fst]
-  case snd => grind [NeutEqTm.snd]
-  case idRec => grind [NeutEqTm.idRec]
-  case conv_neut => grind [NeutEqTm.conv_neut]
-  case clos_tp => grind [ClosEqTp.clos_tp]
-  case clos_val_tp => grind [ClosEqTp.clos_val_tp]
   case clos₂_tp Aeq Beq C ihE _ eq =>
     apply Clos₂EqTp.clos₂_tp (ihE eq) (Aeq.conv_ctx eq) (Beq.conv_ctx _) C
     grind [Clos₂EqTp.clos₂_tp, EqTp.conv_ctx, EqCtx.snoc, EqTp.trans_tp, EqTp.symm_tp]
@@ -444,76 +425,67 @@ theorem conv_ctx :
     exact ClosEqTm.clos_val_tm (env eq) (Aeq.conv_ctx eq)
       (Beq.conv_ctx <| eq.snoc <| EqTp.refl_tp Aeq.wf_right) vb
   case nil eq => exact .nil _ eq.wf_right
-  case snoc => grind [EnvEqSb.snoc]
+  grind_cases
 
--- TODO: name-based grind_cases
-
-theorem ValEqTp.conv_ctx {Γ Γ' l vA A} : ValEqTp Γ l vA A → EqCtx Γ Γ' → ValEqTp Γ' l vA A :=
+theorem ValEqTp.conv_ctx {Γ Γ' l vA A} : ValEqTp E Γ l vA A → EqCtx E Γ Γ' → ValEqTp E Γ' l vA A :=
   fun h eq => _root_.conv_ctx.1 h eq
 
-theorem ValEqTm.conv_ctx {Γ Γ' l vt t A} : ValEqTm Γ l vt t A → EqCtx Γ Γ' →
-    ValEqTm Γ' l vt t A :=
+theorem ValEqTm.conv_ctx {Γ Γ' l vt t A} : ValEqTm E Γ l vt t A → EqCtx E Γ Γ' →
+    ValEqTm E Γ' l vt t A :=
   fun h eq => _root_.conv_ctx.2.1 h eq
 
-theorem NeutEqTm.conv_ctx {Γ Γ' l vt t A} : NeutEqTm Γ l vt t A → EqCtx Γ Γ' →
-    NeutEqTm Γ' l vt t A :=
+theorem NeutEqTm.conv_ctx {Γ Γ' l vt t A} : NeutEqTm E Γ l vt t A → EqCtx E Γ Γ' →
+    NeutEqTm E Γ' l vt t A :=
   fun h eq => _root_.conv_ctx.2.2.1 h eq
 
-theorem ClosEqTp.conv_ctx {Γ Γ' l l' A vB B} : ClosEqTp Γ l l' A vB B → EqCtx Γ Γ' →
-    ClosEqTp Γ' l l' A vB B :=
+theorem ClosEqTp.conv_ctx {Γ Γ' l l' A vB B} : ClosEqTp E Γ l l' A vB B → EqCtx E Γ Γ' →
+    ClosEqTp E Γ' l l' A vB B :=
   fun h eq => _root_.conv_ctx.2.2.2.1 h eq
 
-theorem Clos₂EqTp.conv_ctx {Γ Γ' A B C vC l l' l''} : Clos₂EqTp Γ A l B l' l'' vC C → EqCtx Γ Γ' →
-    Clos₂EqTp Γ' A l B l' l'' vC C :=
+theorem Clos₂EqTp.conv_ctx {Γ Γ' A B C vC l l' l''} :
+    Clos₂EqTp E Γ A l B l' l'' vC C →
+    EqCtx E Γ Γ' →
+    Clos₂EqTp E Γ' A l B l' l'' vC C :=
   fun h eq => _root_.conv_ctx.2.2.2.2.1 h eq
 
 theorem ClosEqTm.conv_ctx {Γ Γ' l l' A B vb b} :
-    ClosEqTm Γ l l' A B vb b → EqCtx Γ Γ' → ClosEqTm Γ' l l' A B vb b :=
+    ClosEqTm E Γ l l' A B vb b → EqCtx E Γ Γ' → ClosEqTm E Γ' l l' A B vb b :=
   fun h eq => _root_.conv_ctx.2.2.2.2.2.1 h eq
 
-theorem EnvEqSb.conv_dom {Δ Δ' E σ Γ} : EnvEqSb Δ E σ Γ → EqCtx Δ Δ' → EnvEqSb Δ' E σ Γ :=
+theorem EnvEqSb.conv_dom {Δ Δ' Eᵥ σ Γ} : EnvEqSb E Δ Eᵥ σ Γ → EqCtx E Δ Δ' → EnvEqSb E Δ' Eᵥ σ Γ :=
   fun h eq => _root_.conv_ctx.2.2.2.2.2.2 h eq
 
 /-! ## Weakening is free -/
 
 theorem wk_all :
-    (∀ {Γ l vA A}, ValEqTp Γ l vA A → ∀ {C k}, Γ ⊢[k] C →
-      ValEqTp ((C,k) :: Γ) l vA (A.subst Expr.wk)) ∧
-    (∀ {Γ l vt t A}, ValEqTm Γ l vt t A → ∀ {C k}, Γ ⊢[k] C →
-      ValEqTm ((C,k) :: Γ) l vt (t.subst Expr.wk) (A.subst Expr.wk)) ∧
-    (∀ {Γ l vt t A}, NeutEqTm Γ l vt t A → ∀ {C k}, Γ ⊢[k] C →
-      NeutEqTm ((C,k) :: Γ) l vt (t.subst Expr.wk) (A.subst Expr.wk)) ∧
-    (∀ {Γ l l' A vB B}, ClosEqTp Γ l l' A vB B → ∀ {C k}, Γ ⊢[k] C →
-      ClosEqTp ((C,k) :: Γ) l l' (A.subst Expr.wk) vB (B.subst (Expr.up Expr.wk))) ∧
-    (∀ {Γ A l B l' l'' vC C}, Clos₂EqTp Γ A l B l' l'' vC C → ∀ {D k}, Γ ⊢[k] D →
-      Clos₂EqTp ((D,k) :: Γ) (A.subst Expr.wk) l (B.subst (Expr.up Expr.wk)) l' l''
+    (∀ {Γ l vA A}, ValEqTp E Γ l vA A → ∀ {C k}, E ∣ Γ ⊢[k] C →
+      ValEqTp E ((C,k) :: Γ) l vA (A.subst Expr.wk)) ∧
+    (∀ {Γ l vt t A}, ValEqTm E Γ l vt t A → ∀ {C k}, E ∣ Γ ⊢[k] C →
+      ValEqTm E ((C,k) :: Γ) l vt (t.subst Expr.wk) (A.subst Expr.wk)) ∧
+    (∀ {Γ l vt t A}, NeutEqTm E Γ l vt t A → ∀ {C k}, E ∣ Γ ⊢[k] C →
+      NeutEqTm E ((C,k) :: Γ) l vt (t.subst Expr.wk) (A.subst Expr.wk)) ∧
+    (∀ {Γ l l' A vB B}, ClosEqTp E Γ l l' A vB B → ∀ {C k}, E ∣ Γ ⊢[k] C →
+      ClosEqTp E ((C,k) :: Γ) l l' (A.subst Expr.wk) vB (B.subst (Expr.up Expr.wk))) ∧
+    (∀ {Γ A l B l' l'' vC C}, Clos₂EqTp E Γ A l B l' l'' vC C → ∀ {D k}, E ∣ Γ ⊢[k] D →
+      Clos₂EqTp E ((D,k) :: Γ) (A.subst Expr.wk) l (B.subst (Expr.up Expr.wk)) l' l''
         vC (C.subst (Expr.up <| Expr.up Expr.wk))) ∧
-    (∀ {Γ l l' A B vb b}, ClosEqTm Γ l l' A B vb b → ∀ {C k}, Γ ⊢[k] C →
-      ClosEqTm ((C,k) :: Γ) l l' (A.subst Expr.wk) (B.subst (Expr.up Expr.wk))
+    (∀ {Γ l l' A B vb b}, ClosEqTm E Γ l l' A B vb b → ∀ {C k}, E ∣ Γ ⊢[k] C →
+      ClosEqTm E ((C,k) :: Γ) l l' (A.subst Expr.wk) (B.subst (Expr.up Expr.wk))
         vb (b.subst (Expr.up Expr.wk))) ∧
-    (∀ {Γ E σ Δ}, EnvEqSb Γ E σ Δ → ∀ {C k}, Γ ⊢[k] C →
-      EnvEqSb ((C,k) :: Γ) E (Expr.comp Expr.wk σ) Δ) := by
+    (∀ {Γ Eᵥ σ Δ}, EnvEqSb E Γ Eᵥ σ Δ → ∀ {C k}, E ∣ Γ ⊢[k] C →
+      EnvEqSb E ((C,k) :: Γ) Eᵥ (Expr.comp Expr.wk σ) Δ) := by
   mutual_induction ValEqTp
   all_goals intros; try dsimp [Expr.subst] at *
-  case pi => grind [ValEqTp.pi]
-  case sigma => grind [ValEqTp.sigma]
-  case Id => grind [ValEqTp.Id]
   case univ => grind [ValEqTp.univ, WfCtx.snoc]
-  case el => grind [ValEqTp.el]
   case conv_tp => grind [ValEqTp.conv_tp, EqTp.subst, WfSb.wk]
-  case lam => grind [ValEqTm.lam]
   case pair B _ _ iht ihu _ _ C =>
     have := B.subst (WfSb.wk C |>.up B.wf_binder)
     apply ValEqTm.pair this (iht C) (autosubst% ihu C)
-  case refl => grind [ValEqTm.refl]
-  case code => grind [ValEqTm.code]
-  case neut_tm => grind [ValEqTm.neut_tm]
   case conv_nf => grind [ValEqTm.conv_nf, EqTp.subst, EqTm.subst, WfSb.wk]
   case bvar Γ lk _ _ C =>
     convert NeutEqTm.bvar (Γ.snoc C) (.succ _ _ lk) using 1; grind
   case app ihA ihf iha _ _ C =>
     exact autosubst% NeutEqTm.app (ihA C) (ihf C) (iha C)
-  case fst => grind [NeutEqTm.fst]
   case snd ih _ _ C =>
     exact autosubst% NeutEqTm.snd (ih C)
   case idRec b _ ihA iha ihM ihr ihh _ _ C =>
@@ -550,88 +522,96 @@ theorem wk_all :
   case snoc =>
     simp only [autosubst] at *
     grind [EnvEqSb.snoc]
+  grind_cases
 
-theorem ValEqTp.wk {Γ l vA A} (h : ValEqTp Γ l vA A) {C k} (hC : Γ ⊢[k] C) :
-    ValEqTp ((C,k) :: Γ) l vA (A.subst Expr.wk) :=
+theorem ValEqTp.wk {Γ l vA A} (h : ValEqTp E Γ l vA A) {C k} (hC : E ∣ Γ ⊢[k] C) :
+    ValEqTp E ((C,k) :: Γ) l vA (A.subst Expr.wk) :=
   wk_all.1 h hC
 
-theorem ValEqTm.wk {Γ l vt t A} (h : ValEqTm Γ l vt t A) {C k} (hC : Γ ⊢[k] C) :
-    ValEqTm ((C,k) :: Γ) l vt (t.subst Expr.wk) (A.subst Expr.wk) :=
+theorem ValEqTm.wk {Γ l vt t A} (h : ValEqTm E Γ l vt t A) {C k} (hC : E ∣ Γ ⊢[k] C) :
+    ValEqTm E ((C,k) :: Γ) l vt (t.subst Expr.wk) (A.subst Expr.wk) :=
   wk_all.2.1 h hC
 
-theorem NeutEqTm.wk {Γ l vn n A} (h : NeutEqTm Γ l vn n A) {C k} (hC : Γ ⊢[k] C) :
-    NeutEqTm ((C,k) :: Γ) l vn (n.subst Expr.wk) (A.subst Expr.wk) :=
+theorem NeutEqTm.wk {Γ l vn n A} (h : NeutEqTm E Γ l vn n A) {C k} (hC : E ∣ Γ ⊢[k] C) :
+    NeutEqTm E ((C,k) :: Γ) l vn (n.subst Expr.wk) (A.subst Expr.wk) :=
   wk_all.2.2.1 h hC
 
-theorem ClosEqTp.wk {Γ l l' A vB B} (h : ClosEqTp Γ l l' A vB B) {C k} (hC : Γ ⊢[k] C) :
-    ClosEqTp ((C,k) :: Γ) l l' (A.subst Expr.wk) vB (B.subst (Expr.up Expr.wk)) :=
+theorem ClosEqTp.wk {Γ l l' A vB B} (h : ClosEqTp E Γ l l' A vB B) {C k} (hC : E ∣ Γ ⊢[k] C) :
+    ClosEqTp E ((C,k) :: Γ) l l' (A.subst Expr.wk) vB (B.subst (Expr.up Expr.wk)) :=
   wk_all.2.2.2.1 h hC
 
-theorem Clos₂EqTp.wk {Γ A l B l' l'' vC C} (h : Clos₂EqTp Γ A l B l' l'' vC C)
-    {D k} (hD : Γ ⊢[k] D) :
-    Clos₂EqTp ((D,k) :: Γ) (A.subst Expr.wk) l (B.subst (Expr.up Expr.wk)) l' l''
+theorem Clos₂EqTp.wk {Γ A l B l' l'' vC C} (h : Clos₂EqTp E Γ A l B l' l'' vC C)
+    {D k} (hD : E ∣ Γ ⊢[k] D) :
+    Clos₂EqTp E ((D,k) :: Γ) (A.subst Expr.wk) l (B.subst (Expr.up Expr.wk)) l' l''
       vC (C.subst (Expr.up (Expr.up Expr.wk))) :=
   wk_all.2.2.2.2.1 h hD
 
-theorem ClosEqTm.wk {Γ l l' A B vb b} (h : ClosEqTm Γ l l' A B vb b) {C k} (hC : Γ ⊢[k] C) :
-    ClosEqTm ((C,k) :: Γ) l l' (A.subst Expr.wk) (B.subst (Expr.up Expr.wk))
+theorem ClosEqTm.wk {Γ l l' A B vb b} (h : ClosEqTm E Γ l l' A B vb b) {C k} (hC : E ∣ Γ ⊢[k] C) :
+    ClosEqTm E ((C,k) :: Γ) l l' (A.subst Expr.wk) (B.subst (Expr.up Expr.wk))
       vb (b.subst (Expr.up Expr.wk)) :=
   wk_all.2.2.2.2.2.1 h hC
 
-theorem EnvEqSb.wk {Δ E σ Γ} (h : EnvEqSb Δ E σ Γ) {C k} (hC : Δ ⊢[k] C) :
-    EnvEqSb ((C,k) :: Δ) E (Expr.comp Expr.wk σ) Γ :=
+theorem EnvEqSb.wk {Δ Eᵥ σ Γ} (h : EnvEqSb E Δ Eᵥ σ Γ) {C k} (hC : E ∣ Δ ⊢[k] C) :
+    EnvEqSb E ((C,k) :: Δ) Eᵥ (Expr.comp Expr.wk σ) Γ :=
   wk_all.2.2.2.2.2.2 h hC
 
 /-! ## Type environments -/
 
 /-- A type environment is a context where all types are in NF. -/
-abbrev TpEnv := List (Val × Nat)
+abbrev TpEnv (χ) := List (Val χ × Nat)
 
-inductive TpEnvEqCtx : TpEnv → Ctx → Prop
+variable (E : Env χ) in
+inductive TpEnvEqCtx : TpEnv χ → Ctx χ → Prop
   | nil : TpEnvEqCtx [] []
   | snoc {vΓ Γ l vA A} :
     TpEnvEqCtx vΓ Γ →
-    ValEqTp Γ l vA A →
+    ValEqTp E Γ l vA A →
     TpEnvEqCtx ((vA, l) :: vΓ) ((A, l) :: Γ)
 
-theorem TpEnvEqCtx.wf_ctx {vΓ Γ} : TpEnvEqCtx vΓ Γ → WfCtx Γ := by
+namespace TpEnvEqCtx
+
+theorem wf_ctx {vΓ Γ} : TpEnvEqCtx E vΓ Γ → WfCtx E Γ := by
   intro vΓ; induction vΓ <;> grind [WfCtx.nil, WfCtx.snoc, ValEqTp.wf_tp]
 
-theorem TpEnvEqCtx.length_eq {vΓ Γ} : TpEnvEqCtx vΓ Γ → vΓ.length = Γ.length := by
+omit [Fact E.Wf] in
+theorem length_eq {vΓ Γ} : TpEnvEqCtx E vΓ Γ → vΓ.length = Γ.length := by
   intro vΓ; induction vΓ <;> simp [*]
 
-theorem TpEnvEqCtx.lt_length {vΓ Γ i A l} : TpEnvEqCtx vΓ Γ → Lookup Γ i A l → i < vΓ.length :=
+omit [Fact E.Wf] in
+theorem lt_length {vΓ Γ i A l} : TpEnvEqCtx E vΓ Γ → Lookup Γ i A l → i < vΓ.length :=
   fun vΓ lk => vΓ.length_eq ▸ lk.lt_length
 
-theorem TpEnvEqCtx.lvl_eq {vΓ Γ i A l} : (h : TpEnvEqCtx vΓ Γ) → (lk : Lookup Γ i A l) →
+omit [Fact E.Wf] in
+theorem lvl_eq {vΓ Γ i A l} : (h : TpEnvEqCtx E vΓ Γ) → (lk : Lookup Γ i A l) →
     (vΓ[i]'(h.lt_length lk)).2 = l := by
   intro h lk
   induction h generalizing i A <;> cases lk <;> grind
-
-theorem TpEnvEqCtx.lookup_wf {vΓ Γ i A l} : (h : TpEnvEqCtx vΓ Γ) → (lk : Lookup Γ i A l) →
-    ValEqTp Γ l (vΓ[i]'(h.lt_length lk)).1 A := by
+theorem lookup_wf {vΓ Γ i A l} : (h : TpEnvEqCtx E vΓ Γ) → (lk : Lookup Γ i A l) →
+    ValEqTp E Γ l (vΓ[i]'(h.lt_length lk)).1 A := by
   intro h lk
   induction h generalizing i A <;> cases lk
   case zero vA => exact vA.wk vA.wf_tp
   case snoc vA ih _ _ lk => exact (ih lk).wk vA.wf_tp
 
+end TpEnvEqCtx
+
 /-! ## Type environments from contexts -/
 
 /-- An identity evaluation environment (i.e., bvars remain themselves)
 for the given type environment. -/
-def envOfTpEnv (vΓ : TpEnv) : List Val :=
+def envOfTpEnv (vΓ : TpEnv χ) : List (Val χ) :=
   vΓ.mapIdx fun i (vA, _) => .neut (.bvar <| vΓ.length - i - 1) vA
 
 @[simp]
-theorem length_envOfTpEnv (vΓ : TpEnv) : (envOfTpEnv vΓ).length = vΓ.length := by
+theorem length_envOfTpEnv (vΓ : TpEnv χ) : (envOfTpEnv vΓ).length = vΓ.length := by
   simp [envOfTpEnv]
 
 @[simp]
-theorem envOfTpEnv_cons (vA : Val) (l : Nat) (vΓ : TpEnv) :
-  envOfTpEnv ((vA, l) :: vΓ) = .neut (.bvar vΓ.length) vA :: envOfTpEnv vΓ := by
+theorem envOfTpEnv_cons (vA : Val χ) (l : Nat) (vΓ : TpEnv χ) :
+    envOfTpEnv ((vA, l) :: vΓ) = .neut (.bvar vΓ.length) vA :: envOfTpEnv vΓ := by
   simp [envOfTpEnv, List.mapIdx_cons]
 
-theorem envOfTpEnv_wf {vΓ Γ} : TpEnvEqCtx vΓ Γ → EnvEqSb Γ (envOfTpEnv vΓ) Expr.bvar Γ := by
+theorem envOfTpEnv_wf {vΓ Γ} : TpEnvEqCtx E vΓ Γ → EnvEqSb E Γ (envOfTpEnv vΓ) Expr.bvar Γ := by
   intro vΓ
   have Γ := vΓ.wf_ctx
   refine EnvEqSb.mk Γ Γ ?_ fun lk => ?_
@@ -642,217 +622,3 @@ theorem envOfTpEnv_wf {vΓ Γ} : TpEnvEqCtx vΓ Γ → EnvEqSb Γ (envOfTpEnv v�
     . rw [vΓ.length_eq]
       apply NeutEqTm.bvar Γ
       exact autosubst% lk
-
-/-! ## Inversion for value relations -/
-
-theorem ValEqTp.inv_pi {Γ C vA vB l k k'} : ValEqTp Γ l (.pi k k' vA vB) C →
-    l = max k k' ∧ ∃ A B, ValEqTp Γ k vA A ∧ ClosEqTp Γ k k' A vB B ∧
-      (Γ ⊢[max k k'] C ≡ .pi k k' A B) := by
-  suffices ∀ {Γ l vC C}, ValEqTp Γ l vC C →
-      ∀ {vA vB k k'}, vC = .pi k k' vA vB →
-        l = max k k' ∧ ∃ A B, ValEqTp Γ k vA A ∧ ClosEqTp Γ k k' A vB B ∧
-        (Γ ⊢[max k k'] C ≡ .pi k k' A B) from
-    fun h => this h rfl
-  mutual_induction ValEqTp
-  all_goals grind [WfTp.pi, ClosEqTp.wf_tp]
-
-theorem ValEqTp.inv_sigma {Γ C vA vB l k k'} : ValEqTp Γ l (.sigma k k' vA vB) C →
-    l = max k k' ∧ ∃ A B, ValEqTp Γ k vA A ∧ ClosEqTp Γ k k' A vB B ∧
-      (Γ ⊢[max k k'] C ≡ .sigma k k' A B) := by
-  suffices ∀ {Γ l vC C}, ValEqTp Γ l vC C →
-      ∀ {vA vB k k'}, vC = .sigma k k' vA vB →
-        l = max k k' ∧ ∃ A B, ValEqTp Γ k vA A ∧ ClosEqTp Γ k k' A vB B ∧
-        (Γ ⊢[max k k'] C ≡ .sigma k k' A B) from
-    fun h => this h rfl
-  mutual_induction ValEqTp
-  all_goals grind [WfTp.sigma, ClosEqTp.wf_tp]
-
-theorem ValEqTp.inv_Id {Γ C vA vt vu l k} : ValEqTp Γ l (.Id k vA vt vu) C →
-    l = k ∧ ∃ A t u,
-      ValEqTp Γ k vA A ∧ ValEqTm Γ k vt t A ∧ ValEqTm Γ k vu u A ∧
-      (Γ ⊢[k] C ≡ .Id k A t u) := by
-  suffices ∀ {Γ l vC C}, ValEqTp Γ l vC C →
-    ∀ {vA vt vu k}, vC = .Id k vA vt vu →
-    l = k ∧ ∃ A t u, ValEqTp Γ k vA A ∧ ValEqTm Γ k vt t A ∧ ValEqTm Γ k vu u A ∧
-      (Γ ⊢[k] C ≡ .Id k A t u) from
-  fun h => this h rfl
-  mutual_induction ValEqTp
-  case Id =>
-    introv vA vt vu
-    have := WfTp.Id vt.wf_tm vu.wf_tm
-    grind [EqTp.refl_tp]
-  all_goals grind
-
-theorem ValEqTp.inv_univ {Γ l k t} : ValEqTp Γ l (.univ k) t → l = k + 1 ∧
-    (Γ ⊢[k + 1] t ≡ .univ k) := by
-  suffices ∀ {Γ l vt t}, ValEqTp Γ l vt t → ∀ {k}, vt = .univ k → l = k + 1 ∧
-      (Γ ⊢[k + 1] t ≡ .univ k) from
-    fun h => this h rfl
-  mutual_induction ValEqTp
-  all_goals grind [WfTp.univ]
-
-theorem ValEqTp.inv_el {Γ l na A} : ValEqTp Γ l (.el na) A →
-    ∃ a, NeutEqTm Γ (l + 1) na a (.univ l) ∧
-      (Γ ⊢[l] A ≡ .el a) := by
-  suffices ∀ {Γ l vA A}, ValEqTp Γ l vA A → ∀ {na}, vA = .el na →
-      ∃ a, NeutEqTm Γ (l + 1) na a (.univ l) ∧
-        (Γ ⊢[l] A ≡ .el a) from
-    fun h => this h rfl
-  mutual_induction ValEqTp
-  all_goals grind [WfTp.el, NeutEqTm.wf_tm]
-
-theorem ValEqTm.inv_lam {Γ C vA vb t l₀ l l'} : ValEqTm Γ l₀ (.lam l l' vA vb) t C →
-    l₀ = max l l' ∧ ∃ A B b,
-      (ValEqTp Γ l vA A) ∧
-      (ClosEqTm Γ l l' A B vb b) ∧
-      (Γ ⊢[max l l'] t ≡ .lam l l' A b : C) ∧
-      (Γ ⊢[max l l'] C ≡ .pi l l' A B) := by
-  suffices
-      ∀ {Γ l₀ vt t C}, ValEqTm Γ l₀ vt t C → ∀ {l l' vA vb}, vt = .lam l l' vA vb →
-        l₀ = max l l' ∧ ∃ A B b, (ValEqTp Γ l vA A) ∧
-          (ClosEqTm Γ l l' A B vb b) ∧
-          (Γ ⊢[max l l'] t ≡ .lam l l' A b : C) ∧
-          (Γ ⊢[max l l'] C ≡ .pi l l' A B) from
-    fun h => this h rfl
-  mutual_induction ValEqTm
-  all_goals intros; try exact True.intro
-  all_goals rename_i eq; cases eq
-  case conv_nf => grind [EqTm.conv_eq]
-  case lam => grind [WfTm.lam, ClosEqTm.wf_tm, WfTm.wf_tp, WfTp.pi]
-
-theorem ValEqTm.inv_pair {Γ C vt vu p l₀ l l'} : ValEqTm Γ l₀ (.pair l l' vt vu) p C →
-    l₀ = max l l' ∧ ∃ A B t u, (ValEqTm Γ l vt t A) ∧ (ValEqTm Γ l' vu u (B.subst t.toSb)) ∧
-      (Γ ⊢[max l l'] p ≡ .pair l l' B t u : C) ∧
-      (Γ ⊢[max l l'] C ≡ .sigma l l' A B) := by
-  suffices
-      ∀ {Γ l₀ vp p C}, ValEqTm Γ l₀ vp p C → ∀ {vt vu l l'}, vp = .pair l l' vt vu →
-        l₀ = max l l' ∧ ∃ A B t u,
-          (ValEqTm Γ l vt t A) ∧
-          (ValEqTm Γ l' vu u (B.subst t.toSb)) ∧
-          (Γ ⊢[max l l'] p ≡ .pair l l' B t u : C) ∧
-          (Γ ⊢[max l l'] C ≡ .sigma l l' A B) from
-    fun h => this h rfl
-  mutual_induction ValEqTm
-  all_goals intros; try exact True.intro
-  all_goals rename_i eq; cases eq
-  case conv_nf => grind [EqTm.conv_eq]
-  case pair => grind [WfTm.pair, ValEqTm.wf_tm, WfTp.sigma]
-
-theorem ValEqTm.inv_refl {Γ C vt r l₀ l} : ValEqTm Γ l₀ (.refl l vt) r C →
-    l₀ = l ∧ ∃ A t, (ValEqTm Γ l vt t A) ∧
-      (Γ ⊢[l] r ≡ .refl l t : C) ∧ (Γ ⊢[l] C ≡ .Id l A t t) := by
-  suffices ∀ {Γ l₀ vr r C}, ValEqTm Γ l₀ vr r C → ∀ {vt l}, vr = .refl l vt → l₀ = l ∧ ∃ A t,
-      (ValEqTm Γ l vt t A) ∧ (Γ ⊢[l] r ≡ .refl l t : C) ∧ (Γ ⊢[l] C ≡ .Id l A t t) from
-    fun h => this h rfl
-  mutual_induction ValEqTm
-  case refl =>
-    introv vt
-    have := vt.wf_tm
-    grind [WfTm.refl, WfTp.Id]
-  all_goals grind [EqTm.conv_eq]
-
-theorem NeutEqTm.inv_idRec {Γ C vA cM va vr nh j l₀ l l'} :
-    NeutEqTm Γ l₀ (.idRec l l' vA va cM vr nh) j C → l₀ = l' ∧ ∃ A M t r u h,
-      (ValEqTp Γ l vA A) ∧
-      (ValEqTm Γ l va t A) ∧
-      (Clos₂EqTp Γ A l (.Id l (A.subst Expr.wk) (t.subst Expr.wk) (.bvar 0)) l l' cM M) ∧
-      (ValEqTm Γ l' vr r (M.subst (.snoc t.toSb <| .refl l t))) ∧
-      (NeutEqTm Γ l nh h (.Id l A t u)) ∧
-      (Γ ⊢[l'] j ≡ .idRec l l' t M r u h : C) ∧
-      (Γ ⊢[l'] C ≡ M.subst (.snoc u.toSb h)) := by
-  suffices
-    ∀ {Γ l₀ vj j C}, NeutEqTm Γ l₀ vj j C → ∀ {vA cM va vr nh l l'},
-      vj = .idRec l l' vA va cM vr nh → l₀ = l' ∧ ∃ A M t r u h,
-        (ValEqTp Γ l vA A) ∧
-        (ValEqTm Γ l va t A) ∧
-        (Clos₂EqTp Γ A l (.Id l (A.subst Expr.wk) (t.subst Expr.wk) (.bvar 0)) l l' cM M) ∧
-        (ValEqTm Γ l' vr r (M.subst (.snoc t.toSb <| .refl l t))) ∧
-        (NeutEqTm Γ l nh h (.Id l A t u)) ∧
-        (Γ ⊢[l'] j ≡ .idRec l l' t M r u h : C) ∧
-        (Γ ⊢[l'] C ≡ M.subst (.snoc u.toSb h)) from
-    fun h => this h rfl
-  mutual_induction ValEqTm
-  case idRec => grind [NeutEqTm.wf_tm, WfTm.wf_tp, → NeutEqTm.idRec]
-  all_goals grind [EqTm.conv_eq]
-
-theorem ValEqTm.inv_code {Γ C vA c l₀} : ValEqTm Γ l₀ (.code vA) c C →
-    ∃ l A, l₀ = l + 1 ∧
-      (ValEqTp Γ l vA A) ∧ (Γ ⊢[l₀] c ≡ .code A : C) ∧ (Γ ⊢[l₀] C ≡ .univ l) := by
-  suffices
-      ∀ {Γ l₀ vc c C}, ValEqTm Γ l₀ vc c C → ∀ {vA}, vc = .code vA →
-        ∃ l A, l₀ = l + 1 ∧
-          (ValEqTp Γ l vA A) ∧ (Γ ⊢[l₀] c ≡ .code A : C) ∧ (Γ ⊢[l₀] C ≡ .univ l) from
-    fun h => this h rfl
-  mutual_induction ValEqTm
-  all_goals intros; try exact True.intro
-  all_goals rename_i eq; cases eq
-  case conv_nf => grind [EqTm.conv_eq]
-  case code => grind [WfTp.univ, WfTm.code, ValEqTp.wf_tp, WfTp.wf_ctx]
-
-theorem ValEqTm.inv_neut {Γ vA A vt t l} : ValEqTm Γ l (.neut vt vA) t A →
-    ValEqTp Γ l vA A ∧ NeutEqTm Γ l vt t A := by
-  suffices ∀ {Γ l vt t A}, ValEqTm Γ l vt t A → ∀ {n vA}, vt = .neut n vA →
-      ValEqTp Γ l vA A ∧ NeutEqTm Γ l n t A from
-    fun h => this h rfl
-  mutual_induction ValEqTm
-  all_goals grind [NeutEqTm.conv_neut, ValEqTp.conv_tp]
-
-theorem NeutEqTm.inv_bvar {Γ A t i l} : NeutEqTm Γ l (.bvar i) t A →
-    ∃ A', Lookup Γ (Γ.length - i - 1) A' l ∧
-      (Γ ⊢[l] t ≡ .bvar (Γ.length - i - 1) : A) ∧ (Γ ⊢[l] A ≡ A') := by
-  suffices ∀ {Γ l vn n A}, NeutEqTm Γ l vn n A → ∀ {i}, vn = .bvar i →
-      ∃ A', Lookup Γ (Γ.length - i - 1) A' l ∧
-        (Γ ⊢[l] n ≡ .bvar (Γ.length - i - 1) : A) ∧ (Γ ⊢[l] A ≡ A') from
-    fun h => this h rfl
-  mutual_induction NeutEqTm
-  all_goals intros; try exact True.intro
-  all_goals rename_i eq; cases eq
-  case bvar Γ _ i _ Γwf lk =>
-    have := lk.lt_length
-    rw [show Γ.length - (Γ.length - i - 1) - 1 = i by omega]
-    exact ⟨_, lk, EqTm.refl_tm (WfTm.bvar (by omega) lk), EqTp.refl_tp (Γwf.lookup_wf lk)⟩
-  case conv_neut => grind [EqTm.conv_eq]
-
-theorem NeutEqTm.inv_app {Γ vA C vf va t l₀ l l'} : NeutEqTm Γ l₀ (.app l l' vA vf va) t C →
-    l₀ = l' ∧ ∃ A B f a,
-      ValEqTp Γ l vA A ∧ NeutEqTm Γ (max l l') vf f (.pi l l' A B) ∧ ValEqTm Γ l va a A ∧
-      (Γ ⊢[l'] t ≡ .app l l' B f a : C) ∧ (Γ ⊢[l'] C ≡ B.subst a.toSb) := by
-  suffices ∀ {Γ l₀ vn n C}, NeutEqTm Γ l₀ vn n C → ∀ {vA vf va l l'}, vn = .app l l' vA vf va →
-      l₀ = l' ∧ ∃ A B f a,
-        ValEqTp Γ l vA A ∧ NeutEqTm Γ (max l l') vf f (.pi l l' A B) ∧ ValEqTm Γ l va a A ∧
-        (Γ ⊢[l'] n ≡ .app l l' B f a : C) ∧ (Γ ⊢[l'] C ≡ B.subst a.toSb) from
-    fun h => this h rfl
-  mutual_induction NeutEqTm
-  all_goals intros; try exact True.intro
-  all_goals rename_i eq; cases eq
-  case conv_neut => grind [EqTm.conv_eq]
-  case app =>
-    grind [WfTm.app, ValEqTm.wf_tm, NeutEqTm.wf_tm, WfSb.toSb, WfTp.subst, WfTp.inv_pi, WfTm.wf_tp]
-
-theorem NeutEqTm.inv_fst {Γ C vp f l₀ l l'} : NeutEqTm Γ l₀ (.fst l l' vp) f C →
-    l₀ = l ∧ ∃ A B p, NeutEqTm Γ (max l l') vp p (.sigma l l' A B) ∧
-      (Γ ⊢[l] f ≡ .fst l l' A B p : C) ∧ (Γ ⊢[l] C ≡ A) := by
-  suffices ∀ {Γ l₀ vn n C}, NeutEqTm Γ l₀ vn n C → ∀ {vp l l'}, vn = .fst l l' vp →
-      l₀ = l ∧ ∃ A B p, NeutEqTm Γ (max l l') vp p (.sigma l l' A B) ∧
-      (Γ ⊢[l] n ≡ .fst l l' A B p : C) ∧ (Γ ⊢[l] C ≡ A) from
-    fun h => this h rfl
-  mutual_induction NeutEqTm
-  all_goals intros; try exact True.intro
-  all_goals rename_i eq; cases eq
-  case conv_neut => grind [EqTm.conv_eq]
-  case fst =>
-    grind [WfTm.fst, NeutEqTm.wf_tm, WfTm.wf_tp, WfTp.inv_sigma, WfTp.wf_ctx, WfCtx.inv_snoc]
-
-theorem NeutEqTm.inv_snd {Γ C vp s l₀ l l'} : NeutEqTm Γ l₀ (.snd l l' vp) s C →
-    l₀ = l' ∧ ∃ A B p, NeutEqTm Γ (max l l') vp p (.sigma l l' A B) ∧
-      (Γ ⊢[l'] s ≡ .snd l l' A B p : C) ∧ (Γ ⊢[l'] C ≡ B.subst (Expr.fst l l' A B p).toSb) := by
-  suffices ∀ {Γ l₀ vn n C}, NeutEqTm Γ l₀ vn n C → ∀ {vp l l'}, vn = .snd l l' vp →
-      l₀ = l' ∧ ∃ A B p, NeutEqTm Γ (max l l') vp p (.sigma l l' A B) ∧
-      (Γ ⊢[l'] n ≡ .snd l l' A B p : C) ∧ (Γ ⊢[l'] C ≡ B.subst (Expr.fst l l' A B p).toSb) from
-    fun h => this h rfl
-  mutual_induction NeutEqTm
-  all_goals intros; try exact True.intro
-  all_goals rename_i eq; cases eq
-  case conv_neut => grind [EqTm.conv_eq]
-  case snd =>
-    grind [WfTm.snd, NeutEqTm.wf_tm, WfTm.wf_tp, WfTp.inv_sigma, WfTp.wf_ctx, WfCtx.inv_snoc]
